Demo.v
@@ -2,9 +2,9 @@ Require Import String.
 Require Import Ast EvalE TCTranslate.
 Require Import List.
 Import ListNotations.
-From Template Require Ast.
-From Template Require Import TemplateMonad.
-From Template Require Import monad_utils.
+From MetaCoq.Template Require Ast.
+From MetaCoq.Template Require Import TemplateMonad.
+From MetaCoq.Template Require Import monad_utils.
 
 
 Import MonadNotation.
@@ -42,7 +42,7 @@ Compute (expr_eval_i 3 Σ [] (indexify [] negb_app_true)).
 
 (* Make a Coq function from the AST of the program *)
 Make Definition coq_negb_app_true :=
-  Eval compute in (expr_to_term Σ (indexify nil negb_app_true)).
+  (expr_to_term Σ (indexify nil negb_app_true)).
 
 Print coq_negb_app_true.
 
@@ -52,7 +52,7 @@ Definition my_negb_syn :=
                    | false -> true  |].
 
 Make Definition my_negb :=
-  Eval compute in (expr_to_term Σ (indexify [] my_negb_syn)).
+  (expr_to_term Σ (indexify [] my_negb_syn)).
 
 Lemma my_negb_coq_negb b :
   my_negb b = negb b.
@@ -60,7 +60,7 @@ Proof. reflexivity. Qed.
 
 Compute (expr_eval_n 3 Σ [] my_negb_syn).
 
-Make Definition coq_my_negb := Eval compute in (expr_to_term Σ (indexify [] my_negb_syn)).
+Make Definition coq_my_negb := (expr_to_term Σ (indexify [] my_negb_syn)).
 
 Import MonadNotation.
 
@@ -94,7 +94,7 @@ Definition is_zero_syn :=
 
   |].
 
-Make Definition is_zero' := Eval compute in (expr_to_term Σ (indexify nil is_zero_syn)).
+Make Definition is_zero' := (expr_to_term Σ (indexify nil is_zero_syn)).
 
 
 Definition pred_syn :=
@@ -107,7 +107,7 @@ Definition pred_syn :=
 
   |].
 
-Make Definition pred' := Eval compute in (expr_to_term Σ (indexify nil pred_syn)).
+Make Definition pred' := (expr_to_term Σ (indexify nil pred_syn)).
 
 Definition prog2 := [| Suc (Suc Z) |].
 
@@ -139,7 +139,7 @@ Definition factorial_syn :=
   |].
 
 Make Definition factorial :=
-  Eval compute in ((expr_to_term Σ (indexify [] factorial_syn))).
+  (expr_to_term Σ (indexify [] factorial_syn)).
 
 Definition plus_syn : expr :=
   [| fix "plus" (x : Nat) : Nat -> Nat :=
@@ -147,7 +147,7 @@ Definition plus_syn : expr :=
            | Z -> \y : Nat -> y
            | Suc y -> \z : Nat -> Suc ("plus" y z) |].
 
-Make Definition my_plus := Eval compute in (expr_to_term Σ (indexify [] plus_syn)).
+Make Definition my_plus := (expr_to_term Σ (indexify [] plus_syn)).
 
 Lemma my_plus_correct n m :
   my_plus n m = n + m.
@@ -167,7 +167,7 @@ Compute (expr_eval_n 10 Σ [] [| {plus_syn} 1 1 |]).
 Definition two_arg_fun_syn := [| \x : Nat -> \y : Bool -> x |].
 
 Make Definition two_arg_fun_app :=
-  Eval compute in (expr_to_term Σ (indexify [] [| {two_arg_fun_syn} 1 true |])).
+  (expr_to_term Σ (indexify [] [| {two_arg_fun_syn} 1 true |])).
 
 Parameter bbb: bool.
 
@@ -185,7 +185,7 @@ Definition plus_syn' :=
   |].
 
 Make Definition my_plus' :=
-  Eval compute in ((expr_to_term Σ (indexify [] plus_syn'))).
+  (expr_to_term Σ (indexify [] plus_syn')).
 
 Lemma my_plus'_0 : forall n, my_plus' 0 n = n.
 Proof.
